vale/code/arch/Vale.Arch.HeapImpl.fst
@@ -17,15 +17,16 @@ noeq type vale_heap_layout_inner : Type u#1 = {
   vl_old_heap:vale_heap;
 }
 
-let empty_vale_heap_layout_inner h = {
-  vl_n_buffers = 0;
-  vl_old_heap = h;
-}
+let empty_vale_heap_layout_inner (h:vale_heap) : vale_heap_layout_inner =
+  {
+    vl_n_buffers = 0;
+    vl_old_heap = h;
+  }
 
 let empty_heaplet (h:vale_heap) (n:nat{n < 16}) : vale_heap =
   let ValeHeap mh ih _ = h in ValeHeap mh ih (Some n)
 
-let empty_vale_heaplets h =
+let empty_vale_heaplets (h:vale_heap) : vale_heaplets =
   Map16.init vale_heap (empty_heaplet h)
 
 let _ih (vh:vale_heap) : GTot interop_heap = Ghost.reveal vh.ih
