vale/code/arch/Vale.Arch.HeapImpl.fsti
@@ -17,7 +17,6 @@ let heaplet_id = n:nat{n < 16}
 
 val vale_heap : Type u#1
 val vale_heap_layout_inner : Type u#1
-val empty_vale_heap_layout_inner (h:vale_heap) : vale_heap_layout_inner
 
 noeq type vale_heap_layout : Type u#1 = {
   vl_inner:vale_heap_layout_inner;
@@ -31,8 +30,6 @@ noeq type vale_full_heap = {
   vf_heap:vale_heap;
   vf_heaplets:vale_heaplets;
 }
-
-val empty_vale_heaplets (h:vale_heap) : vale_heaplets
 
 unfold let full_heap_taint (vfh:vale_full_heap) : memTaint_t =
   vfh.vf_layout.vl_taint
